MyShortHand.v
@@ -5,8 +5,47 @@
 here are some comments
  *)
  
+ Require Import Coq.Classes.EquivDec.
  
+Notation "x =<> y" := ({x = y} + {x <> y}) (at level 100).
+ 
+ Ltac rec_eq :=
+ match goal with
+    | [ x : ?T, y : ?T |- _ ] => 
+       (match T with
+        | nat => generalize nat_eq_eqdec
+        | bool => generalize bool_eqdec
+        | unit => generalize unit_eqdec
+       end) ; 
+       intros X; destruct X with x y as [| paul];
+       try (left; inversion e; subst; reflexivity);
+       try (right; unfold complement in paul; unfold not; 
+            intros Hpaul; apply paul; inversion Hpaul; reflexivity)
+    end.
 
+Ltac eqdecHelper := subst; (left; reflexivity) || (
+right; unfold not; intros; inversion H; contradiction).
+
+Tactic Notation "inv" hyp(H) := inversion H; subst.
+Tactic Notation "cca" := repeat constructor; assumption.
+
+Require Export Coq.Program.Equality.
+Require Export Eqdep_dec.
+Require Export Coq.Arith.EqNat.
+Require Export Coq.Arith.Peano_dec.
+
+Ltac not_eq := let x := fresh "beats" in (let y := fresh "beats" in  ((try right); unfold not; intros x; inversion x as [y];
+     (try (apply inj_pair2_eq_dec in y); auto with eq_dec_db)  )). 
+ (*
+ knowing that a lower level binds more than a higher level. Hence the level for disjunction must be higher than the level for conjunction.
+ Coq < Notation "A /\ B" := (and A B) (at level 80, right associativity).
+Coq < Notation "A \/ B" := (or A B)  (at level 85, right associativity).
+ 
+ *)
+ Print "=".  
+Notation " x = y = z" := (x = y /\ x = z) .
+Notation " x = y = z = a" := (x = y /\ x = z /\ x = a) (at level 200).
+Notation " x = y = z = a = b" := (x = y /\ x = z /\ x = a /\ x = b) (at level 200).
 Tactic Notation "ass" := assumption.
 Tactic Notation "refl" := reflexivity. 
 Tactic Notation "dest" tactic (c) := destruct c .
